aarch64 crefine: make proof generic in irq type size
It turns out that there are platforms with 8-bit wide IRQ types on
AArch64. This means we need the same kind of invariant for VPPIEvent
fault here as we have in ARM_HYP, saying that VPPIEvent only stores IRQs
up to the IRQ bit width, even though the C declares a potentially wider
type.

Signed-off-by: Gerwin Klein <gerwin.klein@proofcraft.systems>

proof/crefine/AARCH64/StateRelation_C.thy
@@ -361,12 +361,25 @@ where
   | "fault_to_H (SeL4_Fault_VPPIEvent irq) lf
           = Some (ArchFault (VPPIEvent (ucast (seL4_Fault_VPPIEvent_CL.irq_w_CL irq))))"
 
+(* On AArch64, the VPPIEvent irq field has enough space to store IRQs of all known platforms (so far
+   up to 9 bits), but there are AArch64 platforms that have a lower IRQ bit width, which is reflected
+   in the abstract type, but not the C type. This means, we need this invariant to argue that the
+   abstract VPPIEvent has enough bit width when reading from the C field. *)
+definition cfault_wf :: "seL4_Fault_CL \<Rightarrow> bool" where
+  "cfault_wf cf \<equiv>
+     case cf of
+       SeL4_Fault_VPPIEvent irq \<Rightarrow> seL4_Fault_VPPIEvent_CL.irq_w_CL irq \<le> mask irq_len
+     | _ \<Rightarrow> True"
+
+lemmas cfault_wf_simps[simp] = cfault_wf_def[split_simps seL4_Fault_CL.split]
+
 definition
   cfault_rel :: "Fault_H.fault option \<Rightarrow> seL4_Fault_CL option \<Rightarrow> lookup_fault_CL option \<Rightarrow> bool"
 where
   "cfault_rel af cf lf \<equiv> \<exists>cf'. cf = Some cf' \<and>
-         (if (is_cap_fault cf') then (\<exists>lf'. lf = Some lf' \<and> fault_to_H cf' lf' = af)
-           else (fault_to_H cf' undefined = af))"
+                               (if is_cap_fault cf'
+                                then \<exists>lf'. lf = Some lf' \<and> fault_to_H cf' lf' = af
+                                else fault_to_H cf' undefined = af \<and> cfault_wf cf')"
 
 definition
   carch_tcb_relation :: "Structures_H.arch_tcb \<Rightarrow> arch_tcb_C \<Rightarrow> bool"
